language_formal/spark2014_semantics/spark2014_core_subset(non-nested)/symboltable.v
@@ -35,18 +35,42 @@ Definition type_decl := Symbol_Table_Module.type_decl.
 Definition proc_decl' := Symbol_Table_Module_X.proc_decl.
 Definition type_decl' := Symbol_Table_Module_X.type_decl.
 
-(*
+Definition level := Symbol_Table_Module.level.
+
+Inductive compile2_flagged_proc_declaration_map: list (idnum * (level * procedure_declaration)) -> 
+                                                 list (idnum * (level * procedure_declaration_x)) -> Prop :=
+    | C2_Flagged_Proc_Declaration_Map_Null:
+        compile2_flagged_proc_declaration_map nil nil
+    | C2_Flagged_Proc_Declaration_Map: forall pd pd' pl pl' p l,
+        compile2_flagged_procedure_declaration pd pd' ->
+        compile2_flagged_proc_declaration_map pl pl' ->
+        compile2_flagged_proc_declaration_map ((p, (l, pd)) :: pl) ((p, (l, pd')) :: pl').
+
+Inductive compile2_flagged_type_declaration_map: list (idnum * type_declaration) -> 
+                                                 list (idnum * type_declaration_x) -> Prop :=
+    | C2_Flagged_Type_Declaration_Map_Null:
+        compile2_flagged_type_declaration_map nil nil
+    | C2_Flagged_Type_Declaration_Map: forall t t' tl tl' x,
+        compile2_flagged_type_declaration t t' ->
+        compile2_flagged_type_declaration_map tl tl' ->
+        compile2_flagged_type_declaration_map ((x, t) :: tl) ((x, t') :: tl').
+
 Inductive compile2_flagged_symbol_table: symbol_table -> symbol_table' -> Prop := 
-  | C2_Flagged_SymTable_Null: forall x,
-      compile2_flagged_symbol_table (mkSymbolTable x nil nil) (mkSymbolTable' x nil nil).
-  | C2  
-.
-*)
+  | C2_Flagged_SymTable: forall p p' t t' x,
+      compile2_flagged_proc_declaration_map p p' ->
+      compile2_flagged_type_declaration_map t t' ->
+      compile2_flagged_symbol_table (mkSymbolTable x p t) (mkSymbolTable' x p' t').
 
 
+(** * Lemmas *)
 
-
-
-
-
+Lemma symbol_table_procedure_rel: forall p st n pb st' n' pb',
+  Symbol_Table_Module.fetch_proc p st = Some (n, pb) ->
+    Symbol_Table_Module_X.fetch_proc p st' = Some (n', pb') ->
+      compile2_flagged_symbol_table st st' ->
+        n = n' /\ compile2_flagged_procedure_declaration pb pb'.
+Proof.
+  intros.
+  admit.
+Qed.
 
