language_formal/spark2014_semantics/spark2014_core_subset(non-nested)/X_SparkTactics.v
@@ -6,7 +6,6 @@ which accompanies this distribution, and is available at
 http://www.eclipse.org/legal/epl-v10.html                             
 *)
 
-Require Export X_Case.
 Require Import X_CpdtTactics.
 
 Create HintDb X_Lib.
@@ -22,30 +21,3 @@ Ltac dup H H' :=
   end.
 
 Ltac smack := try autorewrite with X_Lib in *; crush; eauto.
-
-Tactic Notation "induction" "list" ident(l) :=
-  induction l; [ Case "nil" | Case "cons" ].
-
-Tactic Notation "sub" "induction" "list" ident(l) :=
-  induction l; [ SCase "nil" | SCase "cons" ].
-
-Tactic Notation "sub" "sub" "induction" "list" ident(l) :=
-  induction l; [ SSCase "nil" | SSCase "cons" ].
-
-Tactic Notation "destruct" "list" ident(l) :=
-  destruct l; [ Case "nil" | Case "cons" ].
-
-Tactic Notation "sub" "destruct" "list" ident(l) :=
-  destruct l; [ SCase "nil" | SCase "cons" ].
-
-Tactic Notation "sub" "sub" "destruct" "list" ident(l) :=
-  destruct l; [ SSCase "nil" | SSCase "cons" ].
-
-Tactic Notation "destruct" "option" ident(o) :=
-  destruct o; [ Case "None" | Case "Some" ].
-
-Tactic Notation "sub" "destruct" "option" ident(o) :=
-  destruct o; [ SCase "None" | SCase "Some" ].
-
-Tactic Notation "sub" "sub" "destruct" "option" ident(o) :=
-  destruct o; [ SSCase "None" | SSCase "Some" ].
